restored one-expression version of simulation adequacy

trillium/program_logic/simulation_adequacy_em.v
@@ -9,6 +9,21 @@ Section adequacy.
   Context {LG_EM: LangEM Λ}.
   Context (R: execution_trace Λ → auxiliary_trace M → Prop). 
   
+  Definition wp_premise
+    (Σ: gFunctors)
+    (s: stuckness) (e: expr Λ) σ1 (s1: mstate M)
+    (p: em_init_param)
+    := 
+    (∀ `{Hinv : @IEMGS _ _ LG_EM EM Σ},
+        let _ := IEM_irisG LG_EM EM in
+        let eGS := iem_fairnessGS _ _ in
+        ⊢ (lgem_init_resource ([e], σ1) (lgem_GS0 := iem_phys _ _) ∗
+             em_init_resource s1 p (em_GS0 := iem_fairnessGS _ _)
+           ={⊤}=∗
+              config_wp ∗
+              WP e @ s; locale_of [] e; ⊤ {{ v, em_thread_post (locale_of [] e) v (em_GS0 := eGS) }} ∗
+              rel_always_holds0 R s state_interp (fun v => em_thread_post (locale_of [] e) v (em_GS0 := eGS)) e σ1 s1)).
+
   Definition wp_premise_multiple
     (Σ: gFunctors)
     (s: stuckness) es σ1 (s1: mstate M)
@@ -23,6 +38,16 @@ Section adequacy.
               config_wp ∗
               wptp s es Φs ∗
               rel_always_holds s Φs R (es, σ1) s1)).
+
+  Lemma wp_premise_single Σ
+    s (e1: expr Λ) σ1 s1 p:
+    wp_premise Σ s e1 σ1 s1 p -> wp_premise_multiple Σ s [e1] σ1 s1 p.
+  Proof using.
+    rewrite /wp_premise /wp_premise_multiple.
+    iIntros "%WP1 % [HEAP INIT]".
+    iMod (WP1 Hinv with "[$HEAP $INIT]") as "(CWP & WP1 & RAH)".
+    iFrame. set_solver. 
+  Qed.
 
   Theorem strong_simulation_adequacy_general_multiple
     `{hPre: @IEMGpreS _ _ LG_EM EM Σ}
@@ -166,4 +191,38 @@ Section adequacy.
     apply MATCH. 
   Qed.
   
+  Theorem strong_simulation_adequacy_traces Σ
+    `{hPre: @IEMGpreS _ _ LG_EM EM Σ} (s: stuckness) 
+    (e: expr Λ) σ1 (s1: M)
+    (p: em_init_param)
+    extr
+    (Hvex : extrace_valid extr)
+    (Hexfirst : trfirst extr = ([e], σ1))
+
+    (valid_step: cfg Λ -> olocale Λ → cfg Λ → 
+                 mstate M → mlabel M → mstate M -> Prop)
+    (state_rel: cfg Λ -> mstate M -> Prop)
+    (lbl_rel: olocale Λ -> mlabel M -> Prop)
+    (STEP_LBL_REL: forall c1 oζ c2 δ1 ℓ δ2,
+                 valid_step c1 oζ c2 δ1 ℓ δ2 ->
+                 lbl_rel oζ ℓ)
+    (STEP_MTRANS: forall c1 oζ c2 δ1 ℓ δ2,
+                 valid_step c1 oζ c2 δ1 ℓ δ2 ->
+                 mtrans δ1 ℓ δ2)
+    (R_ST: forall extr mtr, R extr mtr -> state_rel (trace_last extr) (trace_last mtr))
+    (R_STEP: forall extr mtr, R extr mtr -> valid_state_evolution_fairness valid_step extr mtr)
+
+    :
+    rel_finitary R →
+    em_is_init_st ([e], σ1) s1 ->
+    (wp_premise Σ s e σ1 s1 p) ->
+    ∃ (mtr : trace (mstate M) (mlabel M)), 
+      traces_match lbl_rel state_rel locale_step (@mtrans M) extr mtr /\
+      trfirst mtr = s1. 
+  Proof.
+    intros. eapply strong_simulation_adequacy_traces_multiple; last first.
+    { by eapply wp_premise_single. }
+    all: by eauto.
+  Qed.
+
 End adequacy.
